src/Staking/my_token.sol
@@ -1,68 +1,73 @@
 // SPDX-License-Identifier: MIT
 pragma solidity 0.8.20;
+
 import "forge-std/console.sol";
 import "forge-std/interfaces/IERC20.sol";
 
-contract MyToken is IERC20{
-uint256 public totalSupply;
-mapping (address=>uint256)public balanceOf;
-mapping(address => mapping(address => uint)) public allowance;
-address public owner;
-//  string name="my Token";
-    constructor(){
-        owner=msg.sender;
-       // balanceOf[msg.sender]=10**6;
+contract MyToken is IERC20 {
+    uint256 public totalSupply;
+    mapping(address => uint256) public balanceOf;
+    mapping(address => mapping(address => uint256)) public allowance;
+    address public owner;
+    //  string name="my Token";
+
+    constructor() {
+        owner = msg.sender;
+        // balanceOf[msg.sender]=10**6;
     }
-    function transfer(address to, uint256 amount) external returns (bool){
-        balanceOf[msg.sender]-=amount;
-        balanceOf[to]+=amount;
-        emit Transfer(msg.sender,to,amount);
+
+    function transfer(address to, uint256 amount) external returns (bool) {
+        balanceOf[msg.sender] -= amount;
+        balanceOf[to] += amount;
+        emit Transfer(msg.sender, to, amount);
         return true;
     }
-    function approve(address spender, uint256 amount) external returns (bool){
-       allowance[msg.sender][spender]=amount;
-        emit Approval(msg.sender,spender,amount);
-        return true;  
+
+    function approve(address spender, uint256 amount) external returns (bool) {
+        allowance[msg.sender][spender] = amount;
+        emit Approval(msg.sender, spender, amount);
+        return true;
     }
-    function transferFrom(address from, address to, uint256 amount) external returns (bool){
-        allowance[from][msg.sender]-=amount;
-        balanceOf[from]-=amount;
-        balanceOf[to]+=amount;
-        emit Transfer(from,to,amount);
+
+    function transferFrom(address from, address to, uint256 amount) external returns (bool) {
+        allowance[from][msg.sender] -= amount;
+        balanceOf[from] -= amount;
+        balanceOf[to] += amount;
+        emit Transfer(from, to, amount);
         return true;
     }
     //הנפקת מטבע
-    function mint (uint256 amount,address acount)external {
-        balanceOf[msg.sender]+=amount;
-        totalSupply+=amount;
-        emit Transfer(acount, msg.sender, amount);
 
+    function mint(uint256 amount, address acount) external {
+        balanceOf[msg.sender] += amount;
+        totalSupply += amount;
+        emit Transfer(acount, msg.sender, amount);
     }
-   
-     modifier onlyOwner {
+
+    modifier onlyOwner() {
         require(msg.sender == owner, "Only the owner can call this function");
-        console.log('mint',msg.sender);
+        console.log("mint", msg.sender);
         _;
     }
-    //שריפת מטבע 
-    function burn(uint amount) external {
+    //שריפת מטבע
+
+    function burn(uint256 amount) external {
         balanceOf[msg.sender] -= amount;
         totalSupply -= amount;
         emit Transfer(msg.sender, address(0), amount);
     }
-    function name() external pure returns (string memory){
+
+    function name() external pure returns (string memory) {
         return "ygg";
     }
 
     // / @notice Returns the symbol of the token.
-    function symbol() external pure returns (string memory){
+    function symbol() external pure returns (string memory) {
         return "Coin";
     }
 
     /// @notice Returns the decimals places of the token.
-    function  decimals() external pure returns (uint8){
+    function decimals() external pure returns (uint8) {
         return 7;
     }
 }
-
-
