src/Wallet/walletGabaim.sol
@@ -1,5 +1,6 @@
 // SPDX-License-Identifier: MIT
 pragma solidity ^0.8.20;
+
 import "forge-std/console.sol";
 
 contract WalletGabaim {
@@ -7,6 +8,7 @@ contract WalletGabaim {
     //key=address value =1 if is owner or 0 not
     mapping(address => uint256) public myHashTable;
     uint256 balance;
+
     constructor() {
         owner = payable(msg.sender);
         myHashTable[0x5B38Da6a701c568545dCfcB03FcB875f56beddC4] = 1;
@@ -14,25 +16,29 @@ contract WalletGabaim {
         myHashTable[0x4B20993Bc481177ec7E8f571ceCaE8A9e22C02db] = 1;
     }
     //like export in react
+
     receive() external payable {}
+
     function withDraw(uint256 amount) public {
-        require(myHashTable[msg.sender] == 1|| msg.sender==owner, "Only the owner can withdraw");
+        require(myHashTable[msg.sender] == 1 || msg.sender == owner, "Only the owner can withdraw");
         //address(this)=זה הכתובת של הארנק של החוזה
         require(amount <= address(this).balance, "Dont have enough money");
         //מי שבא למשוך הוא אמור לקבל את הכסף
         payable(msg.sender).transfer(amount);
     }
+
     function changeOwners(address newOwner, address oldOwner) public {
         require(msg.sender == owner, "Only the Owner allowed to do this");
         require(myHashTable[newOwner] != 1, "you are owner");
         myHashTable[newOwner] = 1;
         myHashTable[oldOwner] = 0;
     }
+
     function getValue() public view returns (uint256) {
         return address(this).balance;
     }
-    function getGabaim(address hashAddress)public view returns (uint256){
+
+    function getGabaim(address hashAddress) public view returns (uint256) {
         return (myHashTable[hashAddress]);
     }
- 
 }
