src/Wallet/wallet_1.sol
@@ -1,22 +1,25 @@
 // SPDX-License-Identifier: MIT
 pragma solidity >=0.6.12 <0.9.0;
+
 contract wallet {
     address payable public owner;
-    uint256 balance ;
-    constructor(){
-        owner=payable( msg.sender);
+    uint256 balance;
+
+    constructor() {
+        owner = payable(msg.sender);
     }
     //like export in react
-    receive() external payable { }
-   
-   function  withDraw(uint amount)public {
-    require(msg.sender == owner,"Only the owner can withdraw");
-    //address(this)=זה הכתובת של הארנק של החוזה 
-    require(amount<=address(this).balance,"not enough eth in wallet");
-     payable(owner).transfer(amount);  
-  }
-  
-function getValue()external  view returns (uint){
-    return address(this).balance;
-}
+
+    receive() external payable {}
+
+    function withDraw(uint256 amount) public {
+        require(msg.sender == owner, "Only the owner can withdraw");
+        //address(this)=זה הכתובת של הארנק של החוזה
+        require(amount <= address(this).balance, "not enough eth in wallet");
+        payable(owner).transfer(amount);
+    }
+
+    function getValue() external view returns (uint256) {
+        return address(this).balance;
+    }
 }
