src/erc20.sol
@@ -5,10 +5,11 @@ pragma solidity ^0.8.20;
 import "@openzeppelin/contracts/token/ERC20/ERC20.sol";
 
 contract MyToken is ERC20 {
-    constructor() ERC20("MyToken", "Tova"){
+    constructor() ERC20("MyToken", "Tova") {
         this;
     }
-    function mint(address acount,uint256 value)public{
-        mint(acount,value);
+
+    function mint(address acount, uint256 value) public {
+        mint(acount, value);
     }
 }
