test/Acution/acution.t.sol
@@ -1,17 +1,19 @@
-
 // SPDX-License-Identifier: UNLICENSED
 pragma solidity ^0.8.20;
+
 import {Test, console} from "forge-std/Test.sol";
 import "../../src/Acution/acution.sol";
 
-contract Testauction is Test{
-    Auction n ;
-    address user=vm.addr(1);
-    function setUp()public{
-        n=new Auction();
+contract Testauction is Test {
+    Auction n;
+    address user = vm.addr(1);
+
+    function setUp() public {
+        n = new Auction();
     }
-    function testAddSuggest()public{
-        uint suggest=50;
+
+    function testAddSuggest() public {
+        uint256 suggest = 50;
         n.addSuggest(suggest);
     }
 }
