test/Amm/amm.t.sol
@@ -1,48 +1,47 @@
 // SPDX-License-Identifier: UNLICENSED
 pragma solidity ^0.8.20;
+
 import "../../src/Amm/my_tokenA.sol";
 import "../../src/Amm/my_tokenB.sol";
-import"../../src/Amm/amm.sol";
+import "../../src/Amm/amm.sol";
 import {Test, console} from "forge-std/Test.sol";
 
-contract AmmTest is Test{
+contract AmmTest is Test {
     MyTokenA tokenA;
     MyTokenB tokenB;
     Amm amm;
     address user = vm.addr(1);
-    function setUp()public{
 
-        tokenA=new MyTokenA();
-        tokenB=new MyTokenB();
-        amm = new Amm(tokenA,tokenB);
+    function setUp() public {
+        tokenA = new MyTokenA();
+        tokenB = new MyTokenB();
+        amm = new Amm(tokenA, tokenB);
         tokenA.approve(address(amm), 2000000000);
 
-      
         // tokenA.mint(200, user);
         // tokenB.approve(user, 200);
         // tokenB.mint(200, user);
-        
     }
-    function test_Add_notEq()public{
+
+    function test_Add_notEq() public {
         vm.startPrank(user);
-        //אני נותנת הרשאה ל ammלהשתמש בכסף שהנפקתי לטוקנים  
+        //אני נותנת הרשאה ל ammלהשתמש בכסף שהנפקתי לטוקנים
         tokenA.approve(address(amm), 50);
         tokenA.mint(50, user);
         tokenB.approve(user, 100);
         tokenB.mint(100, user);
-        amm.addLiquidity(tokenA.balanceOf(address(user)),tokenB.balanceOf(address(user)));
+        amm.addLiquidity(tokenA.balanceOf(address(user)), tokenB.balanceOf(address(user)));
 
-    // assertEq(amm.balanceUser[msg.sender]==);
-
+        // assertEq(amm.balanceUser[msg.sender]==);
     }
-       function test_Add_Eq()public{
+
+    function test_Add_Eq() public {
         vm.startPrank(user);
-        //אני נותנת הרשאה ל ammלהשתמש בכסף שהנפקתי לטוקנים  
+        //אני נותנת הרשאה ל ammלהשתמש בכסף שהנפקתי לטוקנים
         tokenA.approve(address(amm), 200);
-        amm.addLiquidity(tokenA.balanceOf(address(user)),tokenB.balanceOf(address(user)));
+        amm.addLiquidity(tokenA.balanceOf(address(user)), tokenB.balanceOf(address(user)));
 
-    // assertEq(amm.balanceUser[msg.sender]==);
-
+        // assertEq(amm.balanceUser[msg.sender]==);
     }
-//לא סיימתי לעשות טסטים 
-} 
+    //לא סיימתי לעשות טסטים
+}
