test/Transfer/transfer.t.sol
@@ -1,20 +1,23 @@
 // SPDX-License-Identifier: MIT
-import'../../src/Transfer/transfer.sol';
+import "../../src/Transfer/transfer.sol";
 
 import {Test, console} from "forge-std/Test.sol";
+
 pragma solidity ^0.8.13;
-contract TestTransfer is Test  {
-   
+
+contract TestTransfer is Test {
     Transfer t;
-   function setUp()public{
-        t=new Transfer();
-       payable(address(t)).transfer(50*1e8);
-   } 
-   function test_transfer()public{
-   uint256 eth=50*1e8;
-   uint256 balance;
-   t.send(eth);
-   balance=t.getBalance();
-   assertEq(balance != eth, true);
-   }
+
+    function setUp() public {
+        t = new Transfer();
+        payable(address(t)).transfer(50 * 1e8);
+    }
+
+    function test_transfer() public {
+        uint256 eth = 50 * 1e8;
+        uint256 balance;
+        t.send(eth);
+        balance = t.getBalance();
+        assertEq(balance != eth, true);
+    }
 }
