dafny/src/Ex/lending.dfy
@@ -5,10 +5,20 @@ module Lending {
     import opened Number
     import opened Math
 
-    function Proportion(borrow: real, deposit: real): bool
+    //יחס הניצול -היחס שהוא לוקח בהתאם למשיכות מהבריכה 
+    function utilizationRatio(borrow: real, deposit: real): bool
         requires deposit != 0.0 
-        ensures Proportion(borrow, deposit) == (borrow / deposit <= 0.8) 
+        ensures utilizationRatio(borrow, deposit) == (borrow / deposit <= 0.8) 
     {
         borrow / deposit <= 0.8
     }
+    function  interestMult(utilizationRatio : real ,baseRate:real , annualBorrow:real ) : real
+        requires utilizationRatio != 0.0
+        ensures interestMult(utilizationRatio ,baseRate, annualBorrow) == ((annualBorrow / baseRate) / utilizationRatio > )
+    {
+         
+    }
+
+
+
 }
